cleanup: rework AuthService around `credential_to_principal`

fstar/treesync/symbolic/MLS.TreeSync.Symbolic.AuthService.fst
@@ -5,13 +5,13 @@ open DY.Core
 open DY.Lib
 open MLS.TreeSync.NetworkTypes
 open MLS.TreeSync.Invariants.AuthService
+open MLS.TreeSync.Symbolic.AuthService.CredentialInterpretation
 open MLS.Symbolic
 
 #set-options "--fuel 0 --ifuel 0"
 
 [@@ with_bytes dy_bytes]
 type dy_as_token = {
-  who: principal;
   time: nat;
 }
 
@@ -19,18 +19,38 @@ type dy_as_token = {
 %splice [ps_dy_as_token_is_well_formed] (gen_is_well_formed_lemma (`dy_as_token))
 
 /// Instantiation of the abstract "Authentication Service" for DY*.
-/// The token is a a principal and a timestamp,
+/// The token is a a timestamp,
 /// and the AS attests that the signature verification key belonged to that principal at that time.
 val dy_asp: {|crypto_invariants|} -> trace -> as_parameters dy_bytes
 let dy_asp #ci tr = {
   token_t = dy_as_token;
   credential_ok = (fun (vk, cred) token ->
-    token.time <= (DY.Core.Trace.Base.length tr) /\
-    bytes_invariant (prefix tr token.time) vk /\
-    vk `has_signkey_usage tr` mk_mls_sigkey_usage token.who /\
-    get_signkey_label tr vk == principal_label token.who
+    match credential_to_principal cred with
+    | None -> False
+    | Some who ->
+      token.time <= (DY.Core.Trace.Base.length tr) /\
+      bytes_invariant (prefix tr token.time) vk /\
+      vk `has_signkey_usage (prefix tr token.time)` mk_mls_sigkey_usage who /\
+      get_signkey_label (prefix tr token.time) vk == principal_label who
   );
   valid_successor = (fun (vk_old, cred_old) (vk_new, cred_new) ->
     True
   );
 }
+
+val dy_asp_later:
+  {|crypto_invariants|} ->
+  tr1:trace -> tr2:trace ->
+  inp:as_input bytes -> token:dy_as_token ->
+  Lemma
+  (requires
+    (dy_asp tr1).credential_ok inp token /\
+    tr1 <$ tr2
+  )
+  (ensures (dy_asp tr2).credential_ok inp token)
+  [SMTPat ((dy_asp tr1).credential_ok inp token);
+   SMTPat (tr1 <$ tr2)]
+let dy_asp_later #cinvs tr1 tr2 (vk, cred) token =
+  match credential_to_principal cred with
+  | None -> ()
+  | Some who -> ()
