fstar/treesync/symbolic/MLS.TreeSync.Symbolic.AuthService.CredentialInterpretation.fst
@@ -1,0 +1,9 @@
+module MLS.TreeSync.Symbolic.AuthService.CredentialInterpretation
+
+open Comparse
+
+let credential_to_principal cred =
+  match cred with
+  | C_basic identity ->
+    (ps_prefix_to_ps_whole ps_principal).parse (identity <: bytes)
+  | _ -> None
