fstar/treesync/symbolic/MLS.TreeSync.Symbolic.AuthService.CredentialInterpretation.fsti
@@ -1,0 +1,10 @@
+module MLS.TreeSync.Symbolic.AuthService.CredentialInterpretation
+
+open DY.Core
+open DY.Lib
+open MLS.NetworkTypes
+
+val credential_to_principal:
+  credential_nt bytes ->
+  option principal
+
